Add some reflection for parsers, and a TODO
Based on Adam's work for normalization by evaluation, we implement most
of the infrastructure required to replace the [cbv] calls to the parser
with a single [vm_compute].  Insights include:

- Do normalization on the reified syntax, rather than having a generic
  [Const] constructor and moving unfolded terms into [Const]
- Don't compute separate unfolding info, but instead check unfoldability
  based on whether or not something is headed by constructors.

What remains:
- Setting up a record to hold the reified version of the parser,
  suitable for [vm_compute].
- Setting up the transformation from the reified parser to the
  interpreted parser, in a way that permits a short [cbv] list.
  (Presumably adding an [interp_with_opt] method.)
- Proving soundness of the partial unfolder

src/Common/List/Operations.v
@@ -250,6 +250,30 @@ Module Export List.
            end
        end.
 
+  Fixpoint first_index_partial {A} (f : A -> option bool) (ls : list A) : option (option nat) :=
+    match ls with
+    | nil => Some None
+    | x :: xs =>
+      match f x with
+      | None => None
+      | Some b =>
+        if b then
+          Some (Some 0)
+        else
+          match first_index_partial f xs with
+          | Some (Some i) => Some (Some (S i))
+          | v => v
+          end
+      end
+    end.
+
+  Fixpoint first_index_default_partial {A} (f : A -> option bool) (default : nat) (ls : list A) :=
+    match first_index_partial f ls with
+    | None => None
+    | Some None => Some default
+    | Some v => v
+    end.
+
   Fixpoint sig_In {A} (ls : list A) : list { x : A | List.In x ls }
     := match ls return list { x : A | List.In x ls } with
          | nil => nil
