src/Parsers/Reflective/PartialUnfold.v
@@ -1,0 +1,389 @@
+Require Import Coq.Strings.String Coq.Strings.Ascii.
+Require Import Fiat.Parsers.Reflective.Syntax Fiat.Parsers.Reflective.Semantics.
+Require Import Fiat.Parsers.Reflective.Syntactify.
+Require Import Fiat.Common.
+Require Import Fiat.Common.NatFacts.
+Require Import Fiat.Common.BoolFacts.
+Require Import Fiat.Common.List.Operations.
+Set Implicit Arguments.
+
+Local Open Scope list_scope.
+
+Section normalization_by_evaluation.
+  Context (var : TypeCode -> Type).
+
+  Fixpoint normalized_of (T : TypeCode) : Type :=
+    match T with
+    | csimple T' => Term var T'
+    | carrow A B => normalized_of A -> normalized_of B
+    end.
+
+  Fixpoint reify {T} : normalized_of T -> Term var T
+    := match T return normalized_of T -> Term var T with
+       | csimple _
+         => fun x => x
+       | carrow A B => fun f => RLambda (fun x => reify (f (reflect (RVar x))))
+       end
+  with reflect {T} : Term var T -> normalized_of T
+       := match T return Term var T -> normalized_of T with
+          | csimple _
+            => fun x => x
+          | carrow A B => fun e x => reflect (RApp e (reify x))
+          end.
+
+  Definition onelevel (T : SimpleTypeCode) : Type
+    := interp_SimpleTypeCode_step (Term var) T.
+
+  Definition onelevelG (T : TypeCode) : Type :=
+    match T with
+    | csimple T' => onelevel T'
+    | _ => Empty_set
+    end.
+
+  Inductive args_for_onelevel : TypeCode -> Type :=
+  | an_arg_ol {A B}
+              (arg : option (onelevelG A))
+              (args : args_for_onelevel B)
+    : args_for_onelevel (A --> B)
+  | noargs_ol {T} : args_for_onelevel (csimple T).
+
+  Definition ahdo {A B} (af : args_for_onelevel (A --> B))
+    : option (onelevelG A) :=
+    match af in args_for_onelevel T
+          return match T with
+                 | carrow A B => option (onelevelG A)
+                 | _ => unit
+                 end
+    with
+    | an_arg_ol _ _ arg _ => arg
+    | _ => tt
+    end.
+
+  Definition atlo {A B} (af : args_for_onelevel (A --> B))
+    : args_for_onelevel B :=
+    match af in args_for_onelevel T
+          return match T with
+                 | carrow A B => args_for_onelevel B
+                 | _ => unit
+                 end
+    with
+    | an_arg_ol _ _ _ af' => af'
+    | _ => tt
+    end.
+
+  Section constantOfs.
+    Context (constantOf : forall {T} (t : Term var T), option (onelevelG T)).
+
+    Fixpoint constantOfs {T} (af : args_for var T) : args_for_onelevel T :=
+      match af with
+      | noargs _ => noargs_ol
+      | an_arg _ _ arg af' => an_arg_ol (constantOf arg) (constantOfs af')
+      end.
+  End constantOfs.
+
+  Fixpoint constantOf {T} (t : Term var T) : option (onelevelG T)
+    := match t in Term _ T return option (onelevelG T) with
+       | RLiteralApp _ l af =>
+         match l with
+         | RLC l'
+           => match l' in RLiteralConstructor T return args_for var T -> args_for_onelevel T -> option (onelevel (range_of T)) with
+              | Rpair _ _ => fun af _ => Some (ahd af, ahd (atl af))
+              | RS => fun af afr => option_map S (ahdo afr)
+              | RO => fun _ _ => Some O
+              | Rnil _ => fun _ _ => Some nil
+              | Rcons _ => fun af afr => option_map (cons (ahd af)) (ahdo (atlo afr))
+              | Rfalse => fun _ _ => Some false
+              | Rtrue => fun _ _ => Some true
+              | Rrchar_expr_ascii v
+              | Rstring v
+              | Rritem_ascii v
+                => fun _ _ => Some v
+              end
+         | RLNC _
+           => fun _ _ => None
+         end af (constantOfs (@constantOf) af)
+       | _ => None
+       end.
+
+  Inductive arg_meanings_for : TypeCode -> Type :=
+  | an_argm {A B} (arg : normalized_of A) (args : arg_meanings_for B) : arg_meanings_for (carrow A B)
+  | noargsm {T} : arg_meanings_for (csimple T).
+
+  Definition ahdm {A} {B} (af : arg_meanings_for (A --> B)) : normalized_of A :=
+    match af in arg_meanings_for T return match T with
+                                          | carrow A B => normalized_of A
+                                          | _ => unit
+                                          end with
+    | an_argm _ _ arg _ => arg
+    | _ => tt
+    end.
+
+  Definition atlm {A} {B} (af : arg_meanings_for (A --> B)) : arg_meanings_for B :=
+    match af in arg_meanings_for T return match T with
+                                          | carrow A B => arg_meanings_for B
+                                          | _ => unit
+                                          end with
+    | an_argm _ _ _ af' => af'
+    | _ => tt
+    end.
+
+  Section meanings.
+    Context (meaning : forall {T} (t : Term normalized_of T), normalized_of T).
+
+    Fixpoint meanings {T} (af : args_for normalized_of T) : arg_meanings_for T :=
+      match af with
+      | noargs _ => noargsm
+      | an_arg _ _ arg af' => an_argm (meaning arg) (meanings af')
+      end.
+  End meanings.
+
+  Fixpoint unmeanings {T}
+           (args : arg_meanings_for T)
+    : args_for var T
+    := match args in arg_meanings_for T
+             return args_for _ T
+       with
+       | an_argm _ _ arg args => an_arg (reify arg) (@unmeanings _ args)
+       | noargsm _ => noargs
+       end.
+
+  Fixpoint apply_meaning_helper {P}
+           (af : arg_meanings_for P)
+    : forall (f : normalized_of P),
+      normalized_of (range_of P)
+    := match af in arg_meanings_for P return normalized_of P -> normalized_of (range_of P) with
+       | an_argm _ _ arg args
+         => fun f => @apply_meaning_helper _ args (f arg)
+       | noargsm _ => fun v => v
+       end.
+
+  Fixpoint meaning {T} (t : Term normalized_of T) : normalized_of T.
+  Proof.
+    refine match t in Term _ T return normalized_of T with
+           | RLiteralApp _ l af =>
+             match l with
+             | RLC l'
+               => fun af => RLiteralApp l' (unmeanings af)
+             | RLNC l'
+               => fun af
+                  => match l' in RLiteralNonConstructor T return arg_meanings_for T -> normalized_of (range_of T) -> normalized_of (range_of T) with
+                     | Rfst _ _
+                       => fun af default
+                          => option_rect (fun _ => _)
+                                         fst default
+                                         (constantOf (ahdm af))
+                     | Rsnd _ _
+                       => fun af default
+                          => option_rect (fun _ => _)
+                                         snd default
+                                         (constantOf (ahdm af))
+                     | Rnth' _
+                       => fun af default
+                          => match constantOf (ahdm af), constantOf (ahdm (atlm af)) with
+                             | Some n, Some ls
+                               => List.nth' n ls (ahdm (atlm (atlm af)))
+                             | _, _ => default
+                             end
+                     | Rnth _
+                       => fun af default
+                          => match constantOf (ahdm af), constantOf (ahdm (atlm af)) with
+                             | Some n, Some ls
+                               => List.nth n ls (ahdm (atlm (atlm af)))
+                             | _, _ => default
+                             end
+                     | Rbeq_nat
+                       => fun af default
+                          => match constantOf (ahdm af), constantOf (ahdm (atlm af)) with
+                             | Some n, Some n' =>
+                               syntactify_bool var (EqNat.beq_nat n n')
+                             | _, _ => default
+                             end
+                     | Rmap A B
+                       => fun af default
+                          => option_rect
+                               (fun _ => _)
+                               (fun ls => syntactify_list (List.map (ahdm af) ls))
+                               default
+                               (constantOf (ahdm (atlm af)))
+                     | Rfold_left A B
+                       => fun af default
+                          => option_rect
+                               (fun _ => _)
+                               (fun ls =>
+                                  let init := ahdm (atlm (atlm af)) in
+                                  let f := ahdm af in
+                                  List.fold_left f ls init)
+                               default
+                               (constantOf (ahdm (atlm af)))
+                     | Rorb
+                       => fun af default
+                          => match constantOf (ahdm af) with
+                             | Some b
+                               => if b then syntactify_bool var true else ahdm (atlm af)
+                             | _ => default
+                             end
+                     | Randb
+                       => fun af default
+                          => match constantOf (ahdm af) with
+                             | Some b
+                               => if b then ahdm (atlm af) else syntactify_bool var false
+                             | _ => default
+                             end
+                     | Rorbr
+                       => fun af default
+                          => match constantOf (ahdm (atlm af)) with
+                             | Some b
+                               => if b then syntactify_bool var true else ahdm af
+                             | _ => default
+                             end
+                     | Randbr
+                       => fun af default
+                          => match constantOf (ahdm (atlm af)) with
+                             | Some b
+                               => if b then ahdm af else syntactify_bool var false
+                             | _ => default
+                             end
+                     | Rminusr
+                       => fun af default
+                          => match constantOf (ahdm af), constantOf (ahdm (atlm af)) with
+                             | Some n, Some n'
+                               => syntactify_nat var (minusr n n')
+                             | _, Some n'
+                               => apply_n n' (fun n0 => RLiteralApp Rpred (n0 :: noargs)) (ahdm af)
+                             | _, _ => default
+                             end
+                     | Rpred
+                       => fun af default
+                          => option_rect (fun _ => _)
+                                         (fun n => syntactify_nat var (pred n))
+                                         default
+                                         (constantOf (ahdm af))
+                     | Rlength _
+                       => fun af default
+                          => option_rect (fun _ => _)
+                                         (fun ls => syntactify_nat var (List.length ls))
+                                         default
+                                         (constantOf (ahdm af))
+                     | Rbool_rect_nodep _
+                       => fun af default
+                          => option_rect (fun _ => _)
+                                         (fun b : bool
+                                          => if b
+                                             then ahdm af
+                                             else ahdm (atlm af))
+                                         default
+                                         (constantOf (ahdm (atlm (atlm af))))
+                     | Rlist_rect_nodep A P
+                       => fun af default
+                          => option_rect (fun _ => normalized_of (range_of P))
+                                         (fun ls
+                                          => apply_meaning_helper
+                                               (atlm (atlm (atlm af)))
+                                               (list_rect_nodep
+                                                  (ahdm af)
+                                                  (fun x xs => ahdm (atlm af) x (syntactify_list xs))
+                                                  ls))
+                                         default
+                                         (constantOf (ahdm (atlm (atlm af))))
+                     | Rlist_caset_nodep _ _
+                       => fun af default
+                          => option_rect (fun _ => _)
+                                         (fun ls
+                                          => list_caset_nodep
+                                               (ahdm af)
+                                               (fun x xs => ahdm (atlm af) x (syntactify_list xs))
+                                               ls)
+                                         default
+                                         (constantOf (ahdm (atlm (atlm af))))
+                     | Rleb
+                       => fun af default
+                          => match constantOf (ahdm af), constantOf (ahdm (atlm af)) with
+                             | Some n, Some n' =>
+                               syntactify_bool var (Compare_dec.leb n n')
+                             | _, _ => default
+                             end
+                     | Rcombine _ _
+                       => fun af default
+                          => match constantOf (ahdm af), constantOf (ahdm (atlm af)) with
+                             | Some ls1, Some ls2 =>
+                               syntactify_list
+                                 (List.map
+                                    (fun p => RLiteralApp
+                                                Rpair
+                                                (fst p :: snd p :: noargs))
+                                    (List.combine ls1 ls2))
+                             | _, _ => default
+                             end
+                     | Rrev _
+                       => fun af default
+                          => option_rect (fun _ => _)
+                                         (fun ls => syntactify_list (List.rev ls))
+                                         default
+                                         (constantOf (ahdm af))
+                     | Rup_to
+                       => fun af default
+                          => option_rect (fun _ => _)
+                                         (fun n
+                                          => syntactify_list (List.map (syntactify_nat var) (List.up_to n)))
+                                         default
+                                         (constantOf (ahdm af))
+                     | Rplus
+                       => fun af default
+                          => match constantOf (ahdm af), constantOf (ahdm (atlm af)) with
+                             | Some n, Some n'
+                               => syntactify_nat var (plus n n')
+                             | Some n, _
+                               => apply_n n (fun n0 => RLiteralApp RS (n0 :: noargs)) (ahdm af)
+                             | _, _ => default
+                             end
+                     | Rmax
+                       => fun af default
+                          => match constantOf (ahdm af), constantOf (ahdm (atlm af)) with
+                             | Some n, Some n'
+                               => syntactify_nat var (max n n')
+                             | _, _ => default
+                             end
+                     | Rritem_rect_nodep _
+                       => fun af default
+                          => option_rect (fun _ => _)
+                                         (fun v
+                                          => Reflective.ritem_rect_nodep
+                                               (fun x => ahdm af (syntactify_rchar_expr_ascii var x))
+                                               (fun s => ahdm (atlm af) (syntactify_string var s))
+                                               v)
+                                         default
+                                         (constantOf (ahdm (atlm (atlm af))))
+                     | Rfirst_index_default _
+                       => fun af default
+                          => match constantOf (ahdm (atlm af)), constantOf (ahdm (atlm (atlm af))) with
+                             | Some v, Some ls =>
+                               let f := ahdm af in
+                               match first_index_default_partial (fun a => constantOf (f a)) v ls with
+                               | None => default
+                               | Some n => syntactify_nat var n
+                               end
+                             | _, _ => default
+                             end
+                     | Rinterp_RCharExpr_ascii => fun af default => default
+                     | Rstring_beq
+                       => fun af default
+                          => match constantOf (ahdm af), constantOf (ahdm (atlm af)) with
+                             | Some n, Some n' =>
+                               syntactify_bool var (Equality.string_beq n n')
+                             | _, _ => default
+                             end
+                     (*| Rchar_at_matches => fun af default => default
+                     | Rsplit_string_for_production => fun af default => default*)
+                     end af (RLiteralApp l' (unmeanings af))
+             end (meanings (@meaning) af)
+           | RLambda _ _ f => fun x => @meaning _ (f x)
+           | RVar _ v => v
+           | RApp _ _ f x => @meaning _ f (@meaning _ x)
+           end.
+  Defined.
+
+  Definition normalize {T} (term : Term normalized_of T) : Term var T := reify (meaning term).
+End normalization_by_evaluation.
+
+Definition polynormalize {T} (term : polyTerm T) : polyTerm T
+  := fun var => normalize (term _).
