src/Parsers/Reflective/Semantics.v
@@ -1,0 +1,124 @@
+Require Import Coq.Strings.String Coq.Strings.Ascii.
+Require Import Fiat.Parsers.Reflective.Syntax.
+Require Import Fiat.Common.NatFacts.
+Require Import Fiat.Common.BoolFacts.
+Require Import Fiat.Common.List.Operations.
+Set Implicit Arguments.
+
+Local Open Scope list_scope.
+
+Definition interp_SimpleTypeCode_step
+           (interp_SimpleTypeCode : SimpleTypeCode -> Type)
+           (t : SimpleTypeCode)
+  : Type
+  := match t with
+     | cnat => nat
+     | cbool => bool
+     | cascii => Ascii.ascii
+     | cstring => string
+     | critem_ascii => Reflective.ritem Ascii.ascii
+     | crchar_expr_ascii => Reflective.RCharExpr Ascii.ascii
+     | clist T => list (interp_SimpleTypeCode T)
+     | cprod A B => interp_SimpleTypeCode A * interp_SimpleTypeCode B
+     end%type.
+
+Fixpoint interp_SimpleTypeCode (t : SimpleTypeCode)
+  := interp_SimpleTypeCode_step (@interp_SimpleTypeCode) t.
+
+Fixpoint interp_TypeCode (t : TypeCode) : Type
+  := match t with
+     | csimple T => interp_SimpleTypeCode T
+     | carrow A B => interp_TypeCode A -> interp_TypeCode B
+     end%type.
+
+Definition interp_RLiteralTerm {T} (t : RLiteralTerm T) : interp_TypeCode T
+  := match t with
+     | RLC t'
+       => match t' in (RLiteralConstructor T') return interp_TypeCode T' with
+          | Rpair _ _ => @pair _ _
+          | RS => S
+          | RO => O
+          | Rnil _ => @nil _
+          | Rcons _ => @cons _
+          | Rfalse => false
+          | Rtrue => true
+          | Rrchar_expr_ascii v
+          | Rstring v
+          | Rritem_ascii v
+            => v
+          end
+     | RLNC t'
+       => match t' in (RLiteralNonConstructor T') return interp_TypeCode T' with
+          | Rfst _ _ => @fst _ _
+          | Rsnd _ _ => @snd _ _
+          | Rnth' A => nth'
+          | Rnth A => @List.nth _
+          | Rmap A B => @List.map _ _
+          | Rfold_left A B => @List.fold_left _ _
+          | Rorb => orb
+          | Randb => andb
+          | Randbr => andbr
+          | Rorbr => orbr
+          | Rminusr => minusr
+          | Rpred => pred
+          | Rplus => plus
+          | Rleb => Compare_dec.leb
+          | Rbeq_nat => EqNat.beq_nat
+          | Rstring_beq => Equality.string_beq
+          | Rlength _ => @List.length _
+          | Rbool_rect_nodep _ => @bool_rect_nodep _
+          | Rlist_rect_nodep _ _ => @list_rect_nodep _ _
+          | Rlist_caset_nodep _ _ => @list_caset_nodep _ _
+          | Rritem_rect_nodep _ => @Reflective.ritem_rect_nodep _ _
+          | Rcombine _ _ => @List.combine _ _
+          | Rfirst_index_default _ => @first_index_default _
+          | Rrev _ => @List.rev _
+          | Rup_to => up_to
+          | Rmax => max
+          | Rinterp_RCharExpr_ascii => Reflective.interp_RCharExpr
+          (*| Rchar_at_matches => fun n => char_at_matches n str
+          | Rsplit_string_for_production => fun n => split_string_for_production n str*)
+          end
+     end.
+
+Fixpoint interp_Term {T} (t : Term interp_TypeCode T) : interp_TypeCode T
+  := match t in (Term _ T') return interp_TypeCode T' with
+     | RVar T v => v
+     | RLambda A B f => fun x => @interp_Term _ (f x)
+     | RApp A B f x => @interp_Term _ f (@interp_Term _ x)
+     | RLiteralApp c t args => interp_args_for (interp_RLiteralTerm t) args
+     end
+with interp_args_for {T} (f : interp_TypeCode T)
+                     (args : args_for interp_TypeCode T)
+     : interp_TypeCode (range_of T)
+     := match args in args_for _ T return interp_TypeCode T -> interp_TypeCode (range_of T) with
+        | an_arg A B arg args => fun f => @interp_args_for _ (f (@interp_Term _ arg)) args
+        | noargs T => fun f => f
+        end f.
+
+Section defaulted_fun.
+  Context {var}
+          (interp_var : forall T, var T -> interp_TypeCode T)
+          (uninterp_var : forall T, interp_TypeCode T -> var T).
+
+  Fixpoint interp_Term_fun
+           {T}
+           (t : Term var T) : interp_TypeCode T
+    := match t in (Term _ T') return interp_TypeCode T' with
+       | RVar _ v
+         => interp_var v
+       | RLambda A B f
+         => fun x => @interp_Term_fun _ (f (uninterp_var _ x))
+       | RApp A B f x
+         => @interp_Term_fun
+              _ f
+              (@interp_Term_fun _ x)
+       | RLiteralApp _ t' args
+         => interp_args_for_fun (interp_RLiteralTerm t') args
+       end
+  with interp_args_for_fun {T} (f : interp_TypeCode T) (args : args_for _ T) : interp_TypeCode (range_of T)
+       := match args in args_for _ T return interp_TypeCode T -> interp_TypeCode (range_of T) with
+          | an_arg A B arg args => fun f => interp_args_for_fun (f (interp_Term_fun arg)) args
+          | noargs T => fun f => f
+          end f.
+End defaulted_fun.
