src/Parsers/Reflective/Syntax.v
@@ -1,0 +1,138 @@
+Require Import Coq.Classes.Morphisms. (* for reserved [-->] notation *)
+Require Import Coq.Strings.String Coq.Strings.Ascii.
+Require Import Fiat.Parsers.ContextFreeGrammar.Reflective.
+
+Set Implicit Arguments.
+Delimit Scope typecode_scope with typecode.
+Delimit Scope term_scope with term.
+Delimit Scope termargs_scope with termargs.
+Local Set Boolean Equality Schemes.
+Inductive SimpleTypeCode : Set :=
+| cnat
+| cbool
+| cstring
+| cascii
+| critem_ascii
+| crchar_expr_ascii
+| clist (T : SimpleTypeCode)
+| cprod (A B : SimpleTypeCode).
+Inductive TypeCode : Set :=
+| csimple (T : SimpleTypeCode)
+| carrow (A B : TypeCode).
+Global Coercion csimple : SimpleTypeCode >-> TypeCode.
+Local Unset Boolean Equality Schemes.
+
+Bind Scope typecode_scope with TypeCode.
+Bind Scope typecode_scope with SimpleTypeCode.
+Arguments clist _%typecode.
+Arguments carrow (_ _)%typecode.
+Arguments cprod (_ _)%typecode.
+
+Infix "-->" := carrow : typecode_scope.
+Infix "*" := cprod : typecode_scope.
+
+Fixpoint range_of (T : TypeCode) : SimpleTypeCode
+  := match T with
+     | carrow A B => range_of B
+     | csimple T => T
+     end.
+
+Section term.
+  Context (var : TypeCode -> Type).
+
+  Inductive RLiteralConstructor : TypeCode -> Set :=
+  | Rpair {A B : SimpleTypeCode} : RLiteralConstructor (A --> B --> A * B)
+  | RS : RLiteralConstructor (cnat --> cnat)
+  | RO : RLiteralConstructor cnat
+  | Rnil {A} : RLiteralConstructor (clist A)
+  | Rcons {A : SimpleTypeCode} : RLiteralConstructor (A --> clist A --> clist A)
+  | Rfalse : RLiteralConstructor cbool
+  | Rtrue : RLiteralConstructor cbool
+  | Rrchar_expr_ascii (_ : Reflective.RCharExpr ascii) : RLiteralConstructor crchar_expr_ascii
+  | Rstring (_ : string) : RLiteralConstructor cstring
+  | Rritem_ascii (_ : Reflective.ritem ascii) : RLiteralConstructor critem_ascii.
+  Inductive RLiteralNonConstructor : TypeCode -> Set :=
+  | Rfst {A B} : RLiteralNonConstructor (A * B --> A)
+  | Rsnd {A B} : RLiteralNonConstructor (A * B --> B)
+  | Rnth' {A} : RLiteralNonConstructor (cnat --> clist A --> A --> csimple A)
+  | Rnth {A} : RLiteralNonConstructor (cnat --> clist A --> A --> csimple A)
+  | Rbeq_nat : RLiteralNonConstructor (cnat --> cnat --> cbool)
+  | Rmap {A B : SimpleTypeCode} : RLiteralNonConstructor ((A --> B) --> clist A --> clist B)
+  | Rfold_left {A B : SimpleTypeCode} : RLiteralNonConstructor ((A --> B --> A) --> clist B --> A --> csimple A)
+  | Rorb : RLiteralNonConstructor (cbool --> cbool --> cbool)
+  | Randb : RLiteralNonConstructor (cbool --> cbool --> cbool)
+  | Randbr : RLiteralNonConstructor (cbool --> cbool --> cbool)
+  | Rorbr : RLiteralNonConstructor (cbool --> cbool --> cbool)
+  | Rminusr : RLiteralNonConstructor (cnat --> cnat --> cnat)
+  | Rpred : RLiteralNonConstructor (cnat --> cnat)
+  | Rlength A : RLiteralNonConstructor (clist A --> cnat)
+  | Rbool_rect_nodep {A : SimpleTypeCode} : RLiteralNonConstructor (A --> A --> cbool --> csimple A)
+  | Rlist_rect_nodep {A : SimpleTypeCode} {P : TypeCode} : RLiteralNonConstructor (P --> (A --> clist A --> P --> P) --> clist A --> P)
+  | Rlist_caset_nodep {A P : SimpleTypeCode} : RLiteralNonConstructor (P --> (A --> clist A --> P) --> clist A --> P)
+  | Rleb : RLiteralNonConstructor (cnat --> cnat --> cbool)
+  | Rcombine {A B} : RLiteralNonConstructor (clist A --> clist B --> clist (A * B))
+  | Rrev {A} : RLiteralNonConstructor (clist A --> clist A)
+  | Rup_to : RLiteralNonConstructor (cnat --> clist cnat)
+  | Rplus : RLiteralNonConstructor (cnat --> cnat --> cnat)
+  | Rmax : RLiteralNonConstructor (cnat --> cnat --> cnat)
+  | Rritem_rect_nodep {A : SimpleTypeCode} : RLiteralNonConstructor ((crchar_expr_ascii --> A) --> (cstring --> A) --> critem_ascii --> csimple A)
+  | Rfirst_index_default {A : SimpleTypeCode} : RLiteralNonConstructor ((A --> cbool) --> cnat --> clist A --> cnat)
+  | Rinterp_RCharExpr_ascii : RLiteralNonConstructor (crchar_expr_ascii --> cascii --> cbool)
+  | Rstring_beq : RLiteralNonConstructor (cstring --> cstring --> cbool).
+  (*| Rchar_at_matches
+    : RLiteralNonConstructor (cnat --> (cascii --> cbool) --> cbool)
+  | Rsplit_string_for_production
+    : RLiteralNonConstructor (cnat * (cnat * cnat) --> cnat --> cnat --> (clist cnat)).*)
+
+  Inductive RLiteralTerm (T : TypeCode) : Set :=
+  | RLC (_ : RLiteralConstructor T)
+  | RLNC (_ : RLiteralNonConstructor T).
+
+  Coercion RLC : RLiteralConstructor >-> RLiteralTerm.
+  Coercion RLNC : RLiteralNonConstructor >-> RLiteralTerm.
+
+  Inductive Term : TypeCode -> Type :=
+  | RVar {T} (v : var T) : Term T
+  | RLambda {A B} (f : var A -> Term B)
+    : Term (A --> B)
+  | RApp {A B} (f : Term (A --> B)) (x : Term A)
+    : Term B
+  | RLiteralApp c (t : RLiteralTerm c) (args : args_for c)
+    : Term (range_of c)
+  with args_for : TypeCode -> Type :=
+       | an_arg {A B} (arg : Term A) (args : args_for B) : args_for (A --> B)
+       | noargs {T} : args_for (csimple T).
+  Bind Scope term_scope with Term.
+  Bind Scope termargs_scope with args_for.
+
+  Definition ahd {A B} (af : args_for (A --> B)) : Term A :=
+    match af in args_for T return match T with
+                                  | carrow A B => Term A
+                                  | _ => unit
+                                  end with
+    | an_arg _ _ arg _ => arg
+    | _ => tt
+    end.
+
+  Definition atl {A B} (af : args_for (A --> B)) : args_for B :=
+    match af in args_for T return match T with
+                                  | carrow A B => args_for B
+                                  | _ => unit
+                                  end with
+    | an_arg _ _ _ af' => af'
+    | _ => tt
+    end.
+End term.
+
+Bind Scope term_scope with Term.
+Bind Scope termargs_scope with args_for.
+Arguments RVar {var T%typecode} v.
+Arguments RLambda {var} {A B}%typecode f%term.
+Arguments RApp {var} {A B}%typecode (f x)%term.
+Arguments RLiteralApp {var} {c}%typecode t%term args%termargs.
+Arguments an_arg {var} {A B}%typecode arg%term args%termargs.
+Arguments noargs {var T}.
+
+Infix "::" := an_arg : termargs_scope.
+
+Definition polyTerm T := forall var, Term var T.
